Sudoku/Examples.lean
@@ -14,12 +14,12 @@ theorem one_cell_test_solve (g : Grid) (hg : SudokuRules g)
   unfold one_cell_test
   apply Solvable.Set _ _ (0, 2) 3
   · decide
-  · apply cell_elim hg
+  · apply cell_elim
     intro n hn hn'
     fin_cases hn <;> simp at hn' ⊢
-    · exact row_conflict hg (by decide) hg_0_0
-    · exact row_conflict hg (by decide) hg_0_1
-    · exact row_conflict hg (by decide) hg_0_3
+    · exact row_conflict (by decide) hg_0_0
+    · exact row_conflict (by decide) hg_0_1
+    · exact row_conflict (by decide) hg_0_3
   dsimp [Progress.set', List.get!, List.set]
   apply Solvable.Done
   · decide
@@ -36,43 +36,43 @@ theorem four_by_four_test_solve (g : Grid) (hg : SudokuRules g)
     : Solvable g four_by_four_test := by
   unfold four_by_four_test
   have hg_1_3 : g (1, 3) = 1 := by
-    apply row_elim hg (by decide)
+    apply row_elim (by decide)
     intro b hb
     fin_cases b <;> simp [-ne_eq] at hb ⊢ <;> clear hb
     · simp [hg_1_0]
-    · exact col_conflict hg (by decide) hg_0_1
-    · exact col_conflict hg (by decide) hg_3_2
+    · exact col_conflict (by decide) hg_0_1
+    · exact col_conflict (by decide) hg_3_2
   apply Solvable.Set _ _ _ _ (by decide) hg_1_3
   dsimp [Progress.set', List.get!, List.set]
   have hg_0_3 : g (0, 3) = 2 := by
-    apply col_elim hg (by decide)
+    apply col_elim (by decide)
     intro b hb
     fin_cases b <;> simp [-ne_eq] at hb ⊢ <;> clear hb
     · simp [hg_1_3]
     · simp [hg_2_3]
-    · exact row_conflict hg (by decide) hg_3_1
+    · exact row_conflict (by decide) hg_3_1
   apply Solvable.Set _ _ _ _ (by decide) hg_0_3
   dsimp [Progress.set', List.get!, List.set]
   have hg_1_2 : g (1, 2) = 4 := by
-    apply cell_elim hg
+    apply cell_elim
     intro n hn hn'
     fin_cases hn <;> simp [-ne_eq] at hn' ⊢ <;> first | (absurd hn'; rfl) | clear hn'
-    · exact reg_conflict hg (by decide) (by decide) hg_1_3
-    · exact reg_conflict hg (by decide) (by decide) hg_0_3
-    · exact reg_conflict hg (by decide) (by decide) hg_0_2
+    · exact reg_conflict (by decide) (by decide) hg_1_3
+    · exact reg_conflict (by decide) (by decide) hg_0_3
+    · exact reg_conflict (by decide) (by decide) hg_0_2
   apply Solvable.Set _ _ _ _ (by decide) hg_1_2
   dsimp [Progress.set', List.get!, List.set]
   have hg_3_0 : g (3, 0) = 3 := by
-    apply reg_elim hg (by decide)
+    apply reg_elim (by decide)
     intro c hc
     fin_cases c <;> simp [-ne_eq, reg_coords] at hc ⊢ <;> clear hc
-    · exact row_conflict hg (by decide) hg_2_3
-    · exact row_conflict hg (by decide) hg_2_3
+    · exact row_conflict (by decide) hg_2_3
+    · exact row_conflict (by decide) hg_2_3
     · simp [hg_3_1]
   apply Solvable.Set _ _ _ _ (by decide) hg_3_0
   dsimp [Progress.set', List.get!, List.set]
   have hg_3_3 : g (3, 3) = 4 := by
-    apply row_elim hg (by decide)
+    apply row_elim (by decide)
     intro b hb
     fin_cases b <;> simp [-ne_eq] at hb ⊢ <;> clear hb
     · simp [hg_3_0]
@@ -81,7 +81,7 @@ theorem four_by_four_test_solve (g : Grid) (hg : SudokuRules g)
   apply Solvable.Set _ _ _ _ (by decide) hg_3_3
   dsimp [Progress.set', List.get!, List.set]
   have hg_2_2 : g (2, 2) = 2 := by
-    apply reg_elim hg (by decide)
+    apply reg_elim (by decide)
     intro b hb
     fin_cases b <;> simp [-ne_eq, reg_coords] at hb ⊢ <;> clear hb
     · simp [hg_2_3]
@@ -90,7 +90,7 @@ theorem four_by_four_test_solve (g : Grid) (hg : SudokuRules g)
   apply Solvable.Set _ _ _ _ (by decide) hg_2_2
   dsimp [Progress.set', List.get!, List.set]
   have hg_1_1 : g (1, 1) = 3 := by
-    apply row_elim hg (by decide)
+    apply row_elim (by decide)
     intro b hb
     fin_cases b <;> simp [-ne_eq] at hb ⊢ <;> clear hb
     · simp [hg_1_0]
@@ -99,7 +99,7 @@ theorem four_by_four_test_solve (g : Grid) (hg : SudokuRules g)
   apply Solvable.Set _ _ _ _ (by decide) hg_1_1
   dsimp [Progress.set', List.get!, List.set]
   have hg_2_1 : g (2, 1) = 4 := by
-    apply col_elim hg (by decide)
+    apply col_elim (by decide)
     intro b hb
     fin_cases b <;> simp [-ne_eq] at hb ⊢ <;> clear hb
     · simp [hg_0_1]
@@ -108,7 +108,7 @@ theorem four_by_four_test_solve (g : Grid) (hg : SudokuRules g)
   apply Solvable.Set _ _ _ _ (by decide) hg_2_1
   dsimp [Progress.set', List.get!, List.set]
   have hg_0_0 : g (0, 0) = 4 := by
-    apply row_elim hg (by decide)
+    apply row_elim (by decide)
     intro b hb
     fin_cases b <;> simp [-ne_eq] at hb ⊢ <;> clear hb
     · simp [hg_0_1]
@@ -117,7 +117,7 @@ theorem four_by_four_test_solve (g : Grid) (hg : SudokuRules g)
   apply Solvable.Set _ _ _ _ (by decide) hg_0_0
   dsimp [Progress.set', List.get!, List.set]
   have hg_2_0 : g (2, 0) = 1 := by
-    apply row_elim hg (by decide)
+    apply row_elim (by decide)
     intro b hb
     fin_cases b <;> simp [-ne_eq] at hb ⊢ <;> clear hb
     · simp [hg_2_1]
